Make ctx and adequacy independent of inv

theories/simplang/ctx.v
@@ -2,188 +2,308 @@
 
 From simuliris.simulation Require Import slsls lifting.
 From simuliris.simplang Require Import proofmode tactics.
-From simuliris.simplang Require Import heap_bij log_rel heapbij_refl.
-
-(* TODO: make this file independent of heapbij_refl *)
+From simuliris.simplang Require Import log_rel.
 
 (** First we need to define a notion of "contexts"
 (more general than the 'evaluation contexts' that the language comes with) *)
 Inductive ctx_item :=
-  | LetLCtx (x : binder) (e2 : expr)
-  | LetRCtx (x : binder) (e1 : expr)
-  | CallLCtx (v2 : val)
-  | CallRCtx (e1 : expr)
-  | UnOpCtx (op : un_op)
-  | BinOpLCtx (op : bin_op) (v2 : expr)
-  | BinOpRCtx (op : bin_op) (e1 : expr)
-  | IfLCtx (e1 e2 : expr)
-  | IfMCtx (e0 e2 : expr)
-  | IfRCtx (e0 e1 : expr)
-  | WhileLCtx (e1 : expr)
-  | WhileRCtx (e0 : expr)
-  | PairLCtx (v2 : expr)
-  | PairRCtx (e1 : expr)
-  | FstCtx
-  | SndCtx
-  | InjLCtx
-  | InjRCtx
-  | MatchLCtx (x1 : binder) (e1 : expr) (x2 : binder) (e2 : expr)
-  | MatchMCtx (e0 : expr) (x1 : binder) (x2 : binder) (e2 : expr)
-  | MatchRCtx (e0 : expr) (x1 : binder) (e1 : expr) (x2 : binder)
-  | ForkCtx
-  | AllocNLCtx (v2 : expr)
-  | AllocNRCtx (e1 : expr)
-  | FreeNLCtx (v2 : expr)
-  | FreeNRCtx (e1 : expr)
-  | LoadCtx (o : order)
-  | StoreLCtx (o : order) (v2 : expr)
-  | StoreRCtx (o : order) (e1 : expr)
-  | CmpXchgLCtx (v1 : expr) (v2 : expr)
-  | CmpXchgMCtx (e0 : expr) (v2 : expr)
-  | CmpXchgRCtx (e0 : expr) (e1 : expr)
-  | FaaLCtx (v2 : expr)
-  | FaaRCtx (e1 : expr).
+  | LetLCCtx (x : binder) (e2 : expr)
+  | LetRCCtx (x : binder) (e1 : expr)
+  | CallLCCtx (v2 : val)
+  | CallRCCtx (e1 : expr)
+  | UnOpCCtx (op : un_op)
+  | BinOpLCCtx (op : bin_op) (v2 : expr)
+  | BinOpRCCtx (op : bin_op) (e1 : expr)
+  | IfLCCtx (e1 e2 : expr)
+  | IfMCCtx (e0 e2 : expr)
+  | IfRCCtx (e0 e1 : expr)
+  | WhileLCCtx (e1 : expr)
+  | WhileRCCtx (e0 : expr)
+  | PairLCCtx (v2 : expr)
+  | PairRCCtx (e1 : expr)
+  | FstCCtx
+  | SndCCtx
+  | InjLCCtx
+  | InjRCCtx
+  | MatchLCCtx (x1 : binder) (e1 : expr) (x2 : binder) (e2 : expr)
+  | MatchMCCtx (e0 : expr) (x1 : binder) (x2 : binder) (e2 : expr)
+  | MatchRCCtx (e0 : expr) (x1 : binder) (e1 : expr) (x2 : binder)
+  | ForkCCtx
+  | AllocNLCCtx (v2 : expr)
+  | AllocNRCCtx (e1 : expr)
+  | FreeNLCCtx (v2 : expr)
+  | FreeNRCCtx (e1 : expr)
+  | LoadCCtx (o : order)
+  | StoreLCCtx (o : order) (v2 : expr)
+  | StoreRCCtx (o : order) (e1 : expr)
+  | CmpXchgLCCtx (v1 : expr) (v2 : expr)
+  | CmpXchgMCCtx (e0 : expr) (v2 : expr)
+  | CmpXchgRCCtx (e0 : expr) (e1 : expr)
+  | FaaLCCtx (v2 : expr)
+  | FaaRCCtx (e1 : expr).
 
-Local Definition fill_item (Ci : ctx_item) (e : expr) : expr :=
+Local Definition fill_ctx_item (Ci : ctx_item) (e : expr) : expr :=
   match Ci with
-  | LetLCtx x e2 => Let x e e2
-  | LetRCtx x e1 => Let x e1 e
-  | CallLCtx e2 => Call e e2
-  | CallRCtx e1 => Call e1 e
-  | UnOpCtx op => UnOp op e
-  | BinOpLCtx op e2 => BinOp op e e2
-  | BinOpRCtx op e1 => BinOp op e1 e
-  | IfLCtx e1 e2 => If e e1 e2
-  | IfMCtx e0 e2 => If e0 e e2
-  | IfRCtx e0 e1 => If e0 e1 e
-  | WhileLCtx e1 => While e e1
-  | WhileRCtx e0 => While e0 e
-  | PairLCtx e2 => Pair e e2
-  | PairRCtx e1 => Pair e1 e
-  | FstCtx => Fst e
-  | SndCtx => Snd e
-  | InjLCtx => InjL e
-  | InjRCtx => InjR e
-  | MatchLCtx x1 e1 x2 e2 => Match e x1 e1 x2 e2
-  | MatchMCtx e0 x1 x2 e2 => Match e0 x1 e x2 e2
-  | MatchRCtx e0 x1 e1 x2 => Match e0 x1 e1 x2 e
-  | ForkCtx => Fork e
-  | AllocNLCtx e2 => AllocN e e2
-  | AllocNRCtx e1 => AllocN e1 e
-  | FreeNLCtx e2 => FreeN e e2
-  | FreeNRCtx e1 => FreeN e1 e
-  | LoadCtx o => Load o e
-  | StoreLCtx o e2 => Store o e e2
-  | StoreRCtx o e1 => Store o e1 e
-  | CmpXchgLCtx e1 e2 => CmpXchg e e1 e2
-  | CmpXchgMCtx e0 e2 => CmpXchg e0 e e2
-  | CmpXchgRCtx e0 e1 => CmpXchg e0 e1 e
-  | FaaLCtx e2 => FAA e e2
-  | FaaRCtx e1 => FAA e1 e
+  | LetLCCtx x e2 => Let x e e2
+  | LetRCCtx x e1 => Let x e1 e
+  | CallLCCtx e2 => Call e e2
+  | CallRCCtx e1 => Call e1 e
+  | UnOpCCtx op => UnOp op e
+  | BinOpLCCtx op e2 => BinOp op e e2
+  | BinOpRCCtx op e1 => BinOp op e1 e
+  | IfLCCtx e1 e2 => If e e1 e2
+  | IfMCCtx e0 e2 => If e0 e e2
+  | IfRCCtx e0 e1 => If e0 e1 e
+  | WhileLCCtx e1 => While e e1
+  | WhileRCCtx e0 => While e0 e
+  | PairLCCtx e2 => Pair e e2
+  | PairRCCtx e1 => Pair e1 e
+  | FstCCtx => Fst e
+  | SndCCtx => Snd e
+  | InjLCCtx => InjL e
+  | InjRCCtx => InjR e
+  | MatchLCCtx x1 e1 x2 e2 => Match e x1 e1 x2 e2
+  | MatchMCCtx e0 x1 x2 e2 => Match e0 x1 e x2 e2
+  | MatchRCCtx e0 x1 e1 x2 => Match e0 x1 e1 x2 e
+  | ForkCCtx => Fork e
+  | AllocNLCCtx e2 => AllocN e e2
+  | AllocNRCCtx e1 => AllocN e1 e
+  | FreeNLCCtx e2 => FreeN e e2
+  | FreeNRCCtx e1 => FreeN e1 e
+  | LoadCCtx o => Load o e
+  | StoreLCCtx o e2 => Store o e e2
+  | StoreRCCtx o e1 => Store o e1 e
+  | CmpXchgLCCtx e1 e2 => CmpXchg e e1 e2
+  | CmpXchgMCCtx e0 e2 => CmpXchg e0 e e2
+  | CmpXchgRCCtx e0 e1 => CmpXchg e0 e1 e
+  | FaaLCCtx e2 => FAA e e2
+  | FaaRCCtx e1 => FAA e1 e
   end.
 
 Definition ctx := list ctx_item.
 Definition fill_ctx (C : ctx) (e : expr) : expr :=
-  foldl (flip fill_item) e C.
+  foldl (flip fill_ctx_item) e C.
 
 Lemma fill_ctx_app C1 C2 e :
   fill_ctx (C1 ++ C2) e = fill_ctx C2 (fill_ctx C1 e).
 Proof. apply foldl_app. Qed.
 
-(** Lift our "type system" to contexts. *)
-Definition ctxi_wf (Ci : ctx_item) : Prop :=
-  match Ci with
-  | LetLCtx _ e => expr_wf e
-  | LetRCtx _ e => expr_wf e
-  | CallLCtx e => expr_wf e
-  | CallRCtx e => expr_wf e
-  | UnOpCtx _ => True
-  | BinOpLCtx _ e => expr_wf e
-  | BinOpRCtx _ e => expr_wf e
-  | IfLCtx e1 e2 => expr_wf e1 ∧ expr_wf e2
-  | IfMCtx e0 e2 => expr_wf e0 ∧ expr_wf e2
-  | IfRCtx e0 e1 => expr_wf e0 ∧ expr_wf e1
-  | WhileLCtx e1 => expr_wf e1
-  | WhileRCtx e0 => expr_wf e0
-  | PairLCtx e => expr_wf e
-  | PairRCtx e => expr_wf e
-  | FstCtx | SndCtx | InjLCtx | InjRCtx => True
-  | MatchLCtx _ e1 _ e2 => expr_wf e1 ∧ expr_wf e2
-  | MatchMCtx e0 _ _ e2 => expr_wf e0 ∧ expr_wf e2
-  | MatchRCtx e0 _ e1 _ => expr_wf e0 ∧ expr_wf e1
-  | ForkCtx => True
-  | AllocNLCtx e => expr_wf e
-  | AllocNRCtx e => expr_wf e
-  | FreeNLCtx e => expr_wf e
-  | FreeNRCtx e => expr_wf e
-  | LoadCtx _ => True
-  | StoreLCtx _ e => expr_wf e
-  | StoreRCtx _ e => expr_wf e
-  | CmpXchgLCtx _ _ => False  (* unsupported *)
-  | CmpXchgMCtx _ _ => False  (* unsupported *)
-  | CmpXchgRCtx _ _ => False  (* unsupported *)
-  | FaaLCtx _ => False  (* unsupported *)
-  | FaaRCtx _ => False (* unsupported *)
+Definition sub_exprs (e : expr) : list expr :=
+  match e with
+  | Val v => []
+  | Var x => []
+  | Let x e1 e2 => [e1; e2]
+  | Call e1 e2 => [e1; e2]
+  | UnOp op e => [e]
+  | BinOp op e1 e2 => [e1; e2]
+  | If e0 e1 e2 => [e0;e1;e2]
+  | While e0 e1 => [e0; e1]
+  | Pair e1 e2 => [e1; e2]
+  | Fst e => [e]
+  | Snd e => [e]
+  | InjL e => [e]
+  | InjR e => [e]
+  | Match e0 x1 e1 x2 e2 => [e0;e1;e2]
+  | Fork e => [e]
+  | AllocN e1 e2 => [e1; e2]
+  | FreeN e1 e2 => [e1; e2]
+  | Load o e => [e]
+  | Store o e1 e2 => [e1; e2]
+  | CmpXchg e0 e1 e2 => [e0;e1;e2]
+  | FAA e1 e2 => [e1; e2]
   end.
-Definition ctx_wf : ctx → Prop := Forall ctxi_wf.
 
-Lemma ctx_wf_app C1 C2 :
-  ctx_wf (C1 ++ C2) ↔ ctx_wf C1 ∧ ctx_wf C2.
-Proof. apply Forall_app. Qed.
-Lemma ctx_wf_snoc C Ci :
-  ctx_wf (C ++ [Ci]) ↔ ctx_wf C ∧ ctxi_wf Ci.
-Proof. rewrite ctx_wf_app /ctx_wf Forall_singleton //. Qed.
+Definition expr_same_shape (e1 e2 : expr) : Prop :=
+  match e1, e2 with
+  | Val v1, Val v2 => v1 = v2
+  | Var x1, Var x2 => x1 = x2
+  | Let x1 _ _, Let x2 _ _ => x1 = x2
+  | Call _ _, Call _ _ =>  True
+  | UnOp op1 _, UnOp op2 _ => op1 = op2
+  | BinOp op1 _ _, BinOp op2 _ _ => op1 = op2
+  | If _ _ _, If _ _ _ => True
+  | While _ _, While _ _ => True
+  | Pair _ _, Pair _ _ => True
+  | Fst _, Fst _ => True
+  | Snd _, Snd _ => True
+  | InjL _, InjL _ => True
+  | InjR _, InjR _ => True
+  | Match _ x1 _ y1 _, Match _ x2 _ y2 _ => x1 = x2 ∧ y1 = y2
+  | Fork _, Fork _ => True
+  | AllocN _ _, AllocN _ _ => True
+  | FreeN _ _, FreeN _ _ => True
+  | Load o1 _, Load o2 _ => o1 = o2
+  | Store o1 _ _, Store o2 _ _ => o1 = o2
+  | CmpXchg _ _ _, CmpXchg _ _ _ => True
+  | FAA _ _, FAA _ _ => True
+  | _, _ => False
+  end.
 
-Section ctx.
-  Context `{heapbijG Σ}.
-  Notation log_rel := (log_rel val_rel (const True%I)).
+Fixpoint val_wf (v : val) : Prop :=
+  match v with
+  | LitV (LitLoc l) => False (* no literal locations allowed *)
+  | LitV _ => True
+  | PairV v1 v2 => val_wf v1 ∧ val_wf v2
+  | InjLV v => val_wf v
+  | InjRV v => val_wf v
+  end.
+Section expr_wf.
+  Context (expr_wf : expr → Prop).
+  Fixpoint struct_expr_wf (e : expr) : Prop :=
+    expr_wf e ∧
+    match e with
+    | Val v => True
+    | Var x => True
+    | Let b e1 e2 => struct_expr_wf e1 ∧ struct_expr_wf e2
+    | Call e1 e2 => struct_expr_wf e1 ∧ struct_expr_wf e2
+    | UnOp op e => struct_expr_wf e
+    | BinOp op e1 e2 => struct_expr_wf e1 ∧ struct_expr_wf e2
+    | If e1 e2 e3 => struct_expr_wf e1 ∧ struct_expr_wf e2 ∧ struct_expr_wf e3
+    | While e1 e2 => struct_expr_wf e1 ∧ struct_expr_wf e2
+    | Pair e1 e2 => struct_expr_wf e1 ∧ struct_expr_wf e2
+    | Fst e => struct_expr_wf e
+    | Snd e => struct_expr_wf e
+    | InjL e => struct_expr_wf e
+    | InjR e => struct_expr_wf e
+    | Match e x1 e1 x2 e2 => struct_expr_wf e ∧ struct_expr_wf e1 ∧ struct_expr_wf e2
+    | Fork e => struct_expr_wf e
+    | AllocN e1 e2 => struct_expr_wf e1 ∧ struct_expr_wf e2
+    | FreeN e1 e2 => struct_expr_wf e1 ∧ struct_expr_wf e2
+    | Load o e => struct_expr_wf e
+    | Store o e1 e2 => struct_expr_wf e1 ∧ struct_expr_wf e2
+    | CmpXchg e1 e2 e3 => struct_expr_wf e1 ∧ struct_expr_wf e2 ∧ struct_expr_wf e3
+    | FAA e1 e2 => struct_expr_wf e1 ∧ struct_expr_wf e2
+    end.
+
+  Definition ectxi_wf (Ki : ectx_item) : Prop :=
+    (∀ e, expr_wf (fill_item Ki e)) ∧
+    match Ki with
+    | LetCtx _ e => struct_expr_wf e
+    | CallLCtx v => struct_expr_wf v
+    | CallRCtx e => struct_expr_wf e
+    | UnOpCtx _ => True
+    | BinOpLCtx _ v => struct_expr_wf v
+    | BinOpRCtx _ e => struct_expr_wf e
+    | IfCtx e1 e2 => struct_expr_wf e1 ∧ struct_expr_wf e2
+    | PairLCtx v => struct_expr_wf v
+    | PairRCtx e => struct_expr_wf e
+    | FstCtx | SndCtx | InjLCtx | InjRCtx | LoadCtx _ => True
+    | MatchCtx _ e1 _ e2 => struct_expr_wf e1 ∧ struct_expr_wf e2
+    | AllocNLCtx v => struct_expr_wf v
+    | AllocNRCtx e => struct_expr_wf e
+    | FreeNLCtx v => struct_expr_wf v
+    | FreeNRCtx e => struct_expr_wf e
+    | StoreLCtx _ v => struct_expr_wf v
+    | StoreRCtx _ e => struct_expr_wf e
+    | CmpXchgLCtx v1 v2 => struct_expr_wf v1 ∧ struct_expr_wf v2
+    | CmpXchgMCtx e1 v2 => struct_expr_wf e1 ∧ struct_expr_wf v2
+    | CmpXchgRCtx e1 e2 => struct_expr_wf e1 ∧ struct_expr_wf e2
+    | FaaLCtx v => struct_expr_wf v
+    | FaaRCtx e => struct_expr_wf e
+    end.
+  Definition ectx_wf : ectx → Prop := Forall ectxi_wf.
+
+  Lemma ectx_wf_app C1 C2 :
+    ectx_wf (C1 ++ C2) ↔ ectx_wf C1 ∧ ectx_wf C2.
+  Proof. apply Forall_app. Qed.
+  Lemma ectx_wf_snoc C Ci :
+    ectx_wf (C ++ [Ci]) ↔ ectx_wf C ∧ ectxi_wf Ci.
+  Proof. rewrite ectx_wf_app /ectx_wf Forall_singleton //. Qed.
+
+  (** Lift our "type system" to contexts. *)
+  Definition ctxi_wf (Ci : ctx_item) : Prop :=
+    (∀ e, expr_wf (fill_ctx_item Ci e)) ∧
+    match Ci with
+    | LetLCCtx _ e => struct_expr_wf e
+    | LetRCCtx _ e => struct_expr_wf e
+    | CallLCCtx e => struct_expr_wf e
+    | CallRCCtx e => struct_expr_wf e
+    | UnOpCCtx _ => True
+    | BinOpLCCtx _ e => struct_expr_wf e
+    | BinOpRCCtx _ e => struct_expr_wf e
+    | IfLCCtx e1 e2 => struct_expr_wf e1 ∧ struct_expr_wf e2
+    | IfMCCtx e0 e2 => struct_expr_wf e0 ∧ struct_expr_wf e2
+    | IfRCCtx e0 e1 => struct_expr_wf e0 ∧ struct_expr_wf e1
+    | WhileLCCtx e1 => struct_expr_wf e1
+    | WhileRCCtx e0 => struct_expr_wf e0
+    | PairLCCtx e => struct_expr_wf e
+    | PairRCCtx e => struct_expr_wf e
+    | FstCCtx | SndCCtx | InjLCCtx | InjRCCtx => True
+    | MatchLCCtx _ e1 _ e2 => struct_expr_wf e1 ∧ struct_expr_wf e2
+    | MatchMCCtx e0 _ _ e2 => struct_expr_wf e0 ∧ struct_expr_wf e2
+    | MatchRCCtx e0 _ e1 _ => struct_expr_wf e0 ∧ struct_expr_wf e1
+    | ForkCCtx => True
+    | AllocNLCCtx e => struct_expr_wf e
+    | AllocNRCCtx e => struct_expr_wf e
+    | FreeNLCCtx e => struct_expr_wf e
+    | FreeNRCCtx e => struct_expr_wf e
+    | LoadCCtx _ => True
+    | StoreLCCtx _ e => struct_expr_wf e
+    | StoreRCCtx _ e => struct_expr_wf e
+    | CmpXchgLCCtx e1 e2 => struct_expr_wf e1 ∧ struct_expr_wf e2
+    | CmpXchgMCCtx e1 e2 => struct_expr_wf e1 ∧ struct_expr_wf e2
+    | CmpXchgRCCtx e1 e2 => struct_expr_wf e1 ∧ struct_expr_wf e2
+    | FaaLCCtx e => struct_expr_wf e
+    | FaaRCCtx e => struct_expr_wf e
+    end.
+  Definition ctx_wf : ctx → Prop := Forall ctxi_wf.
+
+  Lemma ctx_wf_app C1 C2 :
+    ctx_wf (C1 ++ C2) ↔ ctx_wf C1 ∧ ctx_wf C2.
+  Proof. apply Forall_app. Qed.
+  Lemma ctx_wf_snoc C Ci :
+    ctx_wf (C ++ [Ci]) ↔ ctx_wf C ∧ ctxi_wf Ci.
+  Proof. rewrite ctx_wf_app /ctx_wf Forall_singleton //. Qed.
+
+  Context `{!sheapGS Σ} `{!sheapInv Σ}.
+  Context (val_rel : val → val → iProp Σ).
+  Context (thread_own : thread_id → iProp Σ).
+  Notation log_rel := (log_rel val_rel thread_own).
+
+  (* TODO: What is a good name for this? *)
+  Definition log_rel_exprs : Prop :=
+    (∀ e_t e_s, expr_wf e_s → expr_same_shape e_t e_s → ([∗list]e_t'; e_s'∈sub_exprs e_t; sub_exprs e_s, log_rel e_t' e_s') -∗ log_rel e_t e_s).
+
+  Theorem log_rel_refl e :
+    log_rel_exprs →
+    struct_expr_wf e → ⊢ log_rel e e.
+  Proof.
+    intros He Hwf.
+    iInduction e as [ ] "IH" forall (Hwf); destruct Hwf; iApply He; try done; simpl.
+    all: try iDestruct ("IH" with "[%]") as "$".
+    all: try iDestruct ("IH1" with "[%]") as "$".
+    all: try iDestruct ("IH2" with "[%]") as "$".
+    all: naive_solver.
+  Qed.
+
+  Theorem log_rel_ectx K e_t e_s :
+    log_rel_exprs →
+    ectx_wf K → log_rel e_t e_s -∗ log_rel (fill K e_t) (fill K e_s).
+  Proof.
+    intros He Hwf. iInduction (K) as [ | Ki K] "IH" using rev_ind; first by eauto.
+    iIntros "Hrel".
+    rewrite ->ectx_wf_snoc in Hwf. destruct Hwf as [Kwf [Hewf Hiwf]].
+    iSpecialize ("IH" with "[//] Hrel").
+    rewrite !fill_app /=. specialize (Hewf (fill K e_s)).
+    destruct Ki; simpl; iApply He => //=; iFrame "IH".
+    all: repeat iSplit; try done.
+    all: iApply log_rel_refl; [done|].
+    all: naive_solver.
+  Qed.
 
   Theorem log_rel_ctx C e_t e_s :
+    log_rel_exprs →
     ctx_wf C → log_rel e_t e_s -∗ log_rel (fill_ctx C e_t) (fill_ctx C e_s).
   Proof.
-    intros Hwf. iInduction (C) as [ | Ci C] "IH" using rev_ind; first by eauto.
+    intros He Hwf. iInduction (C) as [ | Ci C] "IH" using rev_ind; first by eauto.
     iIntros "Hrel".
-    rewrite ->ctx_wf_snoc in Hwf. destruct Hwf as [Kwf Hiwf].
+    rewrite ->ctx_wf_snoc in Hwf. destruct Hwf as [Kwf [Hewf Hiwf]].
     iSpecialize ("IH" with "[//] Hrel").
-    rewrite !fill_ctx_app /=.
-    destruct Ci; simpl.
-    - iApply (log_rel_let with "IH"); iApply expr_wf_sound; apply Hiwf.
-    - iApply (log_rel_let with "[] IH"); iApply expr_wf_sound; apply Hiwf.
-    -
-  Admitted.
-  (*
-      iApply (log_rel_call with "IH"). ; iApply expr_wf_sound; apply Hiwf.
-    - iApply (log_rel_call with "[] IH"); iApply expr_wf_sound; apply Hiwf.
-    - iApply (log_rel_unop with "IH"); iApply expr_wf_sound; apply Hiwf.
-    - iApply (log_rel_binop with "IH"); iApply expr_wf_sound; apply Hiwf.
-    - iApply (log_rel_binop with "[] IH"); iApply expr_wf_sound; apply Hiwf.
-    - iApply (log_rel_if with "IH"); iApply expr_wf_sound; apply Hiwf.
-    - iApply (log_rel_if with "[] IH"); iApply expr_wf_sound; apply Hiwf.
-    - iApply (log_rel_if with "[] [] IH"); iApply expr_wf_sound; apply Hiwf.
-    - iApply (log_rel_while with "IH"); iApply expr_wf_sound; apply Hiwf.
-    - iApply (log_rel_while with "[] IH"); iApply expr_wf_sound; apply Hiwf.
-    - iApply (log_rel_pair with "IH"); iApply expr_wf_sound; apply Hiwf.
-    - iApply (log_rel_pair with "[] IH"); iApply expr_wf_sound; apply Hiwf.
-    - iApply (log_rel_fst with "IH"); iApply expr_wf_sound; apply Hiwf.
-    - iApply (log_rel_snd with "IH"); iApply expr_wf_sound; apply Hiwf.
-    - iApply (log_rel_injl with "IH"); iApply expr_wf_sound; apply Hiwf.
-    - iApply (log_rel_injr with "IH"); iApply expr_wf_sound; apply Hiwf.
-    - iApply (log_rel_match with "IH"); iApply expr_wf_sound; apply Hiwf.
-    - iApply (log_rel_match with "[] IH"); iApply expr_wf_sound; apply Hiwf.
-    - iApply (log_rel_match with "[] [] IH"); iApply expr_wf_sound; apply Hiwf.
-    - iApply (log_rel_fork with "IH"); iApply expr_wf_sound; apply Hiwf.
-    - iApply (log_rel_allocN with "IH"); iApply expr_wf_sound; apply Hiwf.
-    - iApply (log_rel_allocN with "[] IH"); iApply expr_wf_sound; apply Hiwf.
-    - iApply (log_rel_freeN with "IH"); iApply expr_wf_sound; apply Hiwf.
-    - iApply (log_rel_freeN with "[] IH"); iApply expr_wf_sound; apply Hiwf.
-    - iApply (log_rel_load with "IH"); iApply expr_wf_sound; apply Hiwf.
-    - iApply (log_rel_store with "IH"); iApply expr_wf_sound; apply Hiwf.
-    - iApply (log_rel_store with "[] IH"); iApply expr_wf_sound; apply Hiwf.
-    - by destruct Hiwf.
-    - by destruct Hiwf.
-    - by destruct Hiwf.
-    - by destruct Hiwf.
-    - by destruct Hiwf.
+    rewrite !fill_ctx_app /=. specialize (Hewf (fill_ctx C e_s)).
+    destruct Ci; simpl; iApply He => //=; iFrame "IH".
+    all: repeat iSplit; try done.
+    all: iApply log_rel_refl; [done|].
+    all: naive_solver.
   Qed.
-*)
-End ctx.
+
+End expr_wf.
