theories/simplang/heapbij_races_refl.v
@@ -1,82 +1,54 @@
 From simuliris.simulation Require Import slsls lifting.
 From simuliris.simplang Require Import proofmode tactics.
-From simuliris.simplang Require Import parallel_subst heap_bij_races log_rel.
+From simuliris.simplang Require Import parallel_subst heap_bij_races log_rel ctx.
 
 (** * Reflexivity theorem for the heap bijection value relation *)
 
 (** We will only be able to show reflexivity for "well-formed" terms.
 This is basically our 'type system'. Indeed, "no types" really just means
 "everything has the same type". *)
-Fixpoint val_wf (v : val) : Prop :=
-  match v with
-  | LitV (LitLoc l) => False (* no literal locations allowed *)
-  | LitV _ => True
-  | PairV v1 v2 => val_wf v1 ∧ val_wf v2
-  | InjLV v => val_wf v
-  | InjRV v => val_wf v
-  end.
 
-Fixpoint expr_wf (e : expr) : Prop :=
+Definition expr_wf (e : expr) : Prop :=
   match e with
   | Val v => val_wf v
-  | Var x => True
-  | Let b e1 e2 => expr_wf e1 ∧ expr_wf e2
-  | Call e1 e2 => expr_wf e1 ∧ expr_wf e2
-  | UnOp op e => expr_wf e
-  | BinOp op e1 e2 => expr_wf e1 ∧ expr_wf e2
-  | If e1 e2 e3 => expr_wf e1 ∧ expr_wf e2 ∧ expr_wf e3
-  | While e1 e2 => expr_wf e1 ∧ expr_wf e2
-  | Pair e1 e2 => expr_wf e1 ∧ expr_wf e2
-  | Fst e => expr_wf e
-  | Snd e => expr_wf e
-  | InjL e => expr_wf e
-  | InjR e => expr_wf e
-  | Match e x1 e1 x2 e2 => expr_wf e ∧ expr_wf e1 ∧ expr_wf e2
-  | Fork e => expr_wf e
-  | AllocN e1 e2 => expr_wf e1 ∧ expr_wf e2
-  | FreeN e1 e2 => expr_wf e1 ∧ expr_wf e2
-  | Load o e => o ≠ Na2Ord ∧ expr_wf e
-  | Store o e1 e2 => o ≠ Na2Ord ∧ expr_wf e1 ∧ expr_wf e2
+  | Load o e => o ≠ Na2Ord
+  | Store o e1 e2 => o ≠ Na2Ord
   | CmpXchg e1 e2 e3 => False   (* currently not supported *)
   | FAA e1 e2 => False          (* currently not supported *)
+  | _ => True
   end.
 
 Section refl.
   Context `{nabijG Σ}.
-  Notation log_rel := (log_rel val_rel (λ π, na_locs π ∅)) (only parsing).
 
-  Lemma val_wf_sound v : val_wf v → ⊢ val_rel v v.
+  Theorem expr_wf_sound : log_rel_exprs expr_wf val_rel (λ π, na_locs π ∅).
   Proof.
-    intros Hv.
-    iInduction v as [[] | | | ] "IH"; try by (simpl; try iApply "IH").
-    simpl. destruct Hv as [H1 H2]. iSplit; [by iApply "IH" | by iApply "IH1"].
-  Qed.
-
-  Theorem expr_wf_sound e : expr_wf e → ⊢ log_rel e e.
-  Proof.
-    intros Hwf. iInduction e as [ ] "IH" forall (Hwf).
+    intros e_t e_s Hwf Hs. iIntros "IH".
+    destruct e_s, e_t => //=; simpl in Hs; simplify_eq.
+    all: try iDestruct "IH" as "[IH IH1]".
+    all: try iDestruct "IH1" as "[IH1 IH2]".
+    all: try iDestruct "IH2" as "[IH2 IH3]".
     - (* Val *) iApply log_rel_val. by iApply val_wf_sound.
     - (* Var *) by iApply log_rel_var.
-    - (* Let *) destruct Hwf as [Hwf1 Hwf2]. by iApply (log_rel_let with "(IH [//]) (IH1 [//])").
+    - (* Let *) by iApply (log_rel_let with "IH IH1").
     - (* Call *)
-      destruct Hwf as [Hwf1 Hwf2]. iApply (log_rel_call with "(IH [//]) (IH1 [//])").
+      iApply (log_rel_call with "IH IH1").
       by iIntros (???).
-    - (* UnOp *) by iApply (log_rel_unop with "(IH [//])").
-    - (* BinOp *) destruct Hwf as [Hwf1 Hwf2]. by iApply (log_rel_binop with "(IH [//]) (IH1 [//])").
-    - (* If *) destruct Hwf as (Hwf1 & Hwf2 & Hwf3). by iApply (log_rel_if with "(IH [//]) (IH1 [//]) (IH2 [//])").
-    - (* While *) destruct Hwf as (Hwf1 & Hwf2). by iApply (log_rel_while with "(IH [//]) (IH1 [//])").
-    - (* Pairs *) destruct Hwf as (Hwf1 & Hwf2). by iApply (log_rel_pair with "(IH [//]) (IH1 [//])").
-    - (* Fst *) by iApply (log_rel_fst with "(IH [//])").
-    - (* Snd *) by iApply (log_rel_snd with "(IH [//])").
-    - (* InjL *) by iApply (log_rel_injl with "(IH [//])").
-    - (* InjR *) by iApply (log_rel_injr with "(IH [//])").
-    - (* Match *) destruct Hwf as (Hwf1 & Hwf2 & Hwf3).
-      by iApply (log_rel_match with "(IH [//]) (IH1 [//]) (IH2 [//])").
+    - (* UnOp *) by iApply (log_rel_unop with "IH").
+    - (* BinOp *) by iApply (log_rel_binop with "IH IH1").
+    - (* If *) by iApply (log_rel_if with "IH IH1 IH2").
+    - (* While *) by iApply (log_rel_while with "IH IH1").
+    - (* Pairs *) by iApply (log_rel_pair with "IH IH1").
+    - (* Fst *) by iApply (log_rel_fst with "IH").
+    - (* Snd *) by iApply (log_rel_snd with "IH").
+    - (* InjL *) by iApply (log_rel_injl with "IH").
+    - (* InjR *) by iApply (log_rel_injr with "IH").
+    - (* Match *) destruct_and!; simplify_eq. by iApply (log_rel_match with "IH IH1 IH2").
     - (* Fork *)
-      iApply (log_rel_fork with "(IH [//])").
+      iApply (log_rel_fork with "IH").
       iIntros (????) "Ht Hsim Hfork". by iApply (sim_bij_fork with "Ht Hsim").
     - (* AllocN *)
-      destruct Hwf as (Hwf1 & Hwf2). iApply (log_rel_allocN with "(IH [//]) (IH1 [//])").
+      iApply (log_rel_allocN with "IH IH1").
       iIntros (??????) "Ht Hv Hcont".
       target_alloc l_t as "Hl_t" "Ha_t"; first done.
       source_alloc l_s as "Hl_s" "Ha_s"; first done.
@@ -88,20 +60,17 @@ Section refl.
       }
       by iApply "Hcont".
     - (* FreeN *)
-      destruct Hwf as (Hwf1 & Hwf2). iApply (log_rel_freeN with "(IH [//]) (IH1 [//])").
+      iApply (log_rel_freeN with "IH IH1").
       iIntros (??????) "Ht Hv Hcont". by iApply (sim_bij_free with "Hv Ht").
     - (* Load *)
-      destruct Hwf as (? & Hwf2).
-      iApply (log_rel_load with "(IH [//])").
+      iApply (log_rel_load with "IH").
       iIntros (????) "Ht Hv Hcont". iApply (sim_bij_load with "Hv Ht"); [done..|].
       iIntros (??) "H ?". by iApply ("Hcont" with "[$]").
     - (* Store *)
-      destruct Hwf as (? & Hwf1 & Hwf2). iApply (log_rel_store with "(IH [//]) (IH1 [//])").
+      iApply (log_rel_store with "IH IH1").
       iIntros (??????) "Ht Hl Hv Hcont".
       destruct o => //.
       + by iApply (sim_bij_store_sc with "Hl Ht Hv").
       + by iApply (sim_bij_store_na with "Hl Ht Hv").
-    - done.
-    - done.
   Qed.
 End refl.
